boxFree_formula_persistent_exrinsicForces

NCML/IML/Semantics.lean
@@ -19,16 +19,26 @@ namespace IMLKripkeFrame
 
 abbrev World (_ : IMLKripkeFrame κ) := κ
 
-class MRelLifting (M : IMLKripkeFrame κ) where
-  mRel_lifting : ∀ {x₁ x₂ y₂}, M.iRel x₁ x₂ → M.mRel x₂ y₂ → ∃ y₁, M.mRel x₁ y₁ ∧ M.iRel y₁ y₂
+abbrev mRel' {F : IMLKripkeFrame κ} : F.World → F.World → Prop := F.mRel
+infixl:80 " ⊏ " => IMLKripkeFrame.mRel'
+
+abbrev iRel' {F : IMLKripkeFrame κ} : F.World → F.World → Prop := F.iRel
+infixl:80 " ≼ " => IMLKripkeFrame.iRel'
+
+class MRelLifting (F : IMLKripkeFrame κ) where
+  mRel_lifting : ∀ {x₁ x₂ y₂ : F.World}, x₁ ≼ x₂ → x₂ ⊏ y₂ → ∃ y₁, y₁ ≼ y₂ ∧ x₁ ⊏ y₁
 export MRelLifting (mRel_lifting)
+
+class MixConfluent (F : IMLKripkeFrame κ) where
+  mix_confluent : ∀ {x₁ x₂ y₁ : F.World}, x₁ ≼ x₂ → x₁ ⊏ y₁ → ∃ y₂, y₁ ≼ y₂ ∧ x₂ ⊏ y₂
+export MixConfluent (mix_confluent)
 
 end IMLKripkeFrame
 
 
 structure IMLKripkeModel (κ : Type*) [Nonempty κ] extends IMLKripkeFrame κ where
   val : κ → Nat → Prop
-  val_persistent : ∀ {x₁ x₂} {a}, val x₁ a → iRel x₁ x₂ → val x₂ a
+  val_persistent : ∀ {x₁ x₂ : toIMLKripkeFrame.World} {a}, val x₁ a → x₁ ≼ x₂ → val x₂ a
 
 namespace IMLKripkeModel
 
@@ -44,9 +54,9 @@ def ExtrinsicForces {M : IMLKripkeModel κ} (x₁ : M.World) : BDFormula → Pro
   | .falsum    => False
   | .and φ ψ   => M.ExtrinsicForces x₁ φ ∧ M.ExtrinsicForces x₁ ψ
   | .or φ ψ    => M.ExtrinsicForces x₁ φ ∨ M.ExtrinsicForces x₁ ψ
-  | .imply φ ψ => ∀ x₂, M.iRel x₁ x₂ → M.ExtrinsicForces x₂ φ → M.ExtrinsicForces x₂ ψ
-  | .box φ     => ∀ y₁, M.mRel x₁ y₁ → M.ExtrinsicForces y₁ φ
-  | .dia φ     => ∃ y₁, M.mRel x₁ y₁ ∧ M.ExtrinsicForces y₁ φ
+  | .imply φ ψ => ∀ x₂, x₁ ≼ x₂ → M.ExtrinsicForces x₂ φ → M.ExtrinsicForces x₂ ψ
+  | .box φ     => ∀ y₁, x₁ ⊏ y₁ → M.ExtrinsicForces y₁ φ
+  | .dia φ     => ∃ y₁, x₁ ⊏ y₁ ∧ M.ExtrinsicForces y₁ φ
 infixl:80 " ⊩ᵉ " => ExtrinsicForces
 
 @[grind]
@@ -55,12 +65,12 @@ def IntrinsicForces {M : IMLKripkeModel κ} (x₁ : M.World) : BDFormula → Pro
   | .falsum    => False
   | .and φ ψ   => M.IntrinsicForces x₁ φ ∧ M.IntrinsicForces x₁ ψ
   | .or φ ψ    => M.IntrinsicForces x₁ φ ∨ M.IntrinsicForces x₁ ψ
-  | .imply φ ψ => ∀ x₂, M.iRel x₁ x₂ → M.IntrinsicForces x₂ φ → M.IntrinsicForces x₂ ψ
-  | .box φ     => ∀ x₂, M.iRel x₁ x₂ → ∀ y₂, M.iRel x₂ y₂ → M.IntrinsicForces y₂ φ
-  | .dia φ     => ∀ x₂, M.iRel x₁ x₂ → ∃ y₂, M.iRel x₂ y₂ ∧ M.IntrinsicForces y₂ φ
+  | .imply φ ψ => ∀ x₂, x₁ ≼ x₂ → M.IntrinsicForces x₂ φ → M.IntrinsicForces x₂ ψ
+  | .box φ     => ∀ x₂, x₁ ≼ x₂ → ∀ y₂, x₂ ⊏ y₂ → M.IntrinsicForces y₂ φ
+  | .dia φ     => ∀ x₂, x₁ ≼ x₂ → ∃ y₂, x₂ ⊏ y₂ ∧ M.IntrinsicForces y₂ φ
 infixl:80 " ⊩ⁱ " => IntrinsicForces
 
-lemma formula_persistent_intrinsicForces : x₁ ⊩ⁱ φ → M.iRel x₁ x₂ → x₂ ⊩ⁱ φ := by
+lemma formula_persistent_intrinsicForces : x₁ ⊩ⁱ φ → x₁ ≼ x₂ → x₂ ⊩ⁱ φ := by
   intro h Ix₁x₂;
   induction φ generalizing x₂ with
   | atom a => apply M.val_persistent h Ix₁x₂;
@@ -76,8 +86,7 @@ lemma formula_persistent_intrinsicForces : x₁ ⊩ⁱ φ → M.iRel x₁ x₂ �
     use y₁;
   | _ => grind;
 
-lemma diaFree_formula_persistent_exrinsicForces [M.MRelLifting] (hφ : φ.diaFree) : x₁ ⊩ᵉ φ → M.iRel x₁ x₂ → x₂ ⊩ᵉ φ
-  := by
+lemma diaFree_formula_persistent_exrinsicForces [M.MRelLifting] (hφ : φ.diaFree) : x₁ ⊩ᵉ φ → x₁ ≼ x₂ → x₂ ⊩ᵉ φ := by
   intro h Ix₁x₂;
   induction φ generalizing x₁ x₂ with
   | atom a => apply M.val_persistent h Ix₁x₂;
@@ -87,8 +96,24 @@ lemma diaFree_formula_persistent_exrinsicForces [M.MRelLifting] (hφ : φ.diaFre
     apply h x₃ (Trans.trans Ix₁x₂ Ix₂x₃) hx₃φ;
   | box φ ihφ =>
     intro y₂ Mx₂y₂;
-    obtain ⟨y₁, Mx₁y₁, Iy₁y₂⟩ := M.mRel_lifting Ix₁x₂ Mx₂y₂;
+    obtain ⟨y₁, Iy₁y₂, Mx₁y₁⟩ := M.mRel_lifting Ix₁x₂ Mx₂y₂;
     apply ihφ (by grind) (h y₁ Mx₁y₁) Iy₁y₂;
+
+lemma boxFree_formula_persistent_exrinsicForces [M.MixConfluent] (hφ : φ.boxFree) : x₁ ⊩ᵉ φ → x₁ ≼ x₂ → x₂ ⊩ᵉ φ := by
+  intro h Ix₁x₂;
+  induction φ generalizing x₁ x₂ with
+  | atom a => apply M.val_persistent h Ix₁x₂;
+  | and | or | falsum | box => grind;
+  | imply φ ψ ihφ ihψ =>
+    intro x₃ Ix₂x₃ hx₃φ;
+    apply h x₃ (Trans.trans Ix₁x₂ Ix₂x₃) hx₃φ;
+  | dia φ ihφ =>
+    obtain ⟨y₁, Mx₁y₁, hy₁⟩ := h;
+    obtain ⟨y₂, Iy₁y₂, My₁y₂⟩ := M.mix_confluent Ix₁x₂ Mx₁y₁;
+    use y₂;
+    constructor;
+    . assumption;
+    . exact ihφ (by grind) hy₁ Iy₁y₂;
 
 end IMLKripkeModel
 
